co-induction

coq/my_cpdt/Coinductive.v
@@ -29,7 +29,7 @@ Fixpoint approx A (s : stream A) (n : nat) : list A :=
   match n with
   | O => nil
   | S n' =>
-    match s with 
+    match s with
     | Cons h t => h :: approx t n'
     end
   end.
@@ -133,7 +133,7 @@ Section stream_eq_coind.
   Variable R : stream A -> stream A -> Prop.
   Hypothesis Cons_case_hd : forall s1 s2, R s1 s2 -> hd s1 = hd s2.
   Hypothesis Cons_case_tl : forall s1 s2, R s1 s2 -> R (tl s1) (tl s2).
-  
+
   Theorem stream_eq_coind : forall s1 s2, R s1 s2 -> stream_eq s1 s2.
   Proof.
     cofix stream_eq_coind; destruct s1; destruct s2; intro.
@@ -146,16 +146,221 @@ End stream_eq_coind.
 
 Print stream_eq_coind.
 
-  Theorem ones_eq'' : stream_eq ones ones'.
-  Proof. 
-    apply (stream_eq_coind (fun s1 s2 => s1 = ones /\ s2 = ones')); intros.
-    - crush. (* TODO: what does thid do? *)
-    - crush.
-    - crush.
+Theorem ones_eq'' : stream_eq ones ones'.
+Proof.
+  apply (stream_eq_coind (fun s1 s2 => s1 = ones /\ s2 = ones')); intros.
+  - destruct H. rewrite H. rewrite H0. simpl. reflexivity.
+  - destruct H. split. rewrite H. simpl. reflexivity.
+    rewrite H0. simpl. unfold zeroes. cbv. auto.
+  - auto.
+Qed.
+
+Section stream_eq_loop.
+  Variable A : Type.
+  Variables s1 s2 : stream A.
+
+  Hypothesis Cons_case_hd : hd s1 = hd s2.
+  Hypothesis loop1 : tl s1 = s1.
+  Hypothesis loop2 : tl s2 = s2.
+
+  Theorem stream_eq_loop : stream_eq s1 s2.
+  Proof.
+    apply (stream_eq_coind (fun s1' s2' => s1' = s1 /\ s2' = s2)); crush.
   Qed.
+End stream_eq_loop.
+
+Theorem ones_eq''' : stream_eq ones ones'.
+Proof.
+  apply stream_eq_loop.
+  - simpl. reflexivity.
+  - simpl. reflexivity.
+  - simpl. reflexivity.
+Qed.
+
+Require Import Arith.
+Print fact.
+
+CoFixpoint fact_slow' (n : nat) :=
+  Cons (fact n) (fact_slow' (S n)).
+Definition fact_slow := fact_slow' 1.
+
+CoFixpoint fact_iter' (cur acc : nat) :=
+  Cons acc (fact_iter' (S cur) (acc * cur)).
+Definition fact_iter := fact_iter' 2 1.
+
+Eval simpl in approx fact_iter 5.
+Eval simpl in approx fact_slow 5.
+
+Lemma fact_def : forall x n,
+  fact_iter' x (fact n * S n) =
+  fact_iter' x (fact (S n)).
+Proof.
+  intros. simpl. f_equal. ring.
+Qed.
+
+Hint Resolve fact_def.
+
+(* introducing an existential quantifier for the shared param n *)
+
+(* XXX: Why need an existential here? *)
+
+Lemma fact_eq' : forall n, stream_eq (fact_iter' (S n) (fact n)) (fact_slow' n).
+Proof.
+  intros.
+  apply (stream_eq_coind
+    (fun s1 s2 => exists n, s1 = fact_iter' (S n) (fact n) /\ s2 = fact_slow' n)); crush; eauto.
+Qed.
+
+Theorem fact_eq : stream_eq fact_iter fact_slow.
+  apply fact_eq'.
+Qed.
+
+Section stream_eq_onequant.
+  Variables A B : Type.
+  Variable f g : A -> stream B.
+
+  Hypothesis Cons_case_hd : forall x, hd (f x) = hd (g x).
+  Hypothesis Cons_case_tl : forall x, exists y, tl (f x) = f y /\ tl (g x) = g y.
+
+  Theorem stream_eq_onequant : forall x, stream_eq (f x) (g x).
+  Proof.
+    intros.
+    apply (stream_eq_coind (fun s1 s2 => exists x, s1 = f x /\ s2 = g x)); intros.
+    - destruct H. destruct H. rewrite H. rewrite H0.
+      apply Cons_case_hd.
+    - destruct H. destruct H. rewrite H. rewrite H0.
+      apply Cons_case_tl.
+    - exists x. auto.
+  Qed.
+End stream_eq_onequant.
+
+Lemma fact_eq'' : forall n, stream_eq (fact_iter' (S n) (fact n)) (fact_slow' n).
+  apply stream_eq_onequant; crush; eauto.
+Qed.
+
+(* Simple Modeling of Non-Terminating Programs *)
+
+(* Co-inductive big-step operational semantics *)
+
+Definition var := nat.
+
+Definition vars := var -> nat.
+
+Definition set (vs : vars) (v : var) (n : nat) : vars :=
+  fun v' => if beq_nat v v' then n else vs v'.
+
+Inductive exp : Set :=
+| Const : nat -> exp
+| Var : var -> exp
+| Plus : exp -> exp -> exp
+.
+
+Fixpoint evalExp (vs : vars) (e : exp) : nat :=
+  match e with
+  | Const n => n
+  | Var v => vs v
+  | Plus e1 e2 => evalExp vs e1 + evalExp vs e2
+  end.
+
+Inductive cmd : Set :=
+| Assign : var -> exp -> cmd
+| Seq : cmd -> cmd -> cmd
+| While : exp -> cmd -> cmd.
+
+CoInductive evalCmd : vars -> cmd -> vars -> Prop :=
+| EvalAssign : forall vs v e,
+    evalCmd vs (Assign v e) (set vs v (evalExp vs e))
+| EvalSeq : forall vs1 vs2 vs3 c1 c2,
+    evalCmd vs1 c1 vs2 ->
+    evalCmd vs2 c2 vs3 ->
+    evalCmd vs1 (Seq c1 c2) vs3
+| EvalWhileFalse : forall vs e c,
+    evalExp vs e = 0 ->
+    evalCmd vs (While e c) vs
+| EvalWhileTrue : forall vs1 vs2 vs3 e c,
+    evalExp vs1 e <> 0 ->
+    evalCmd vs1 c vs2 ->
+    evalCmd vs2 (While e c) vs3 ->
+    evalCmd vs1 (While e c) vs3.
+
+(* build co-induction principles *)
+
+Section evalCmd_coind.
+  Variable R : vars -> cmd -> vars -> Prop.
+
+  Hypothesis AssignCase : forall vs1 vs2 v e,
+    R vs1 (Assign v e) vs2 ->
+    vs2 = set vs1 v (evalExp vs1 e).
+
+  Hypothesis SeqCase : forall vs1 vs3 c1 c2,
+    R vs1 (Seq c1 c2) vs3 ->
+    exists vs2, R vs1 c1 vs2 /\ R vs2 c2 vs3.
+
+  Hypothesis WhileCase : forall vs1 vs3 e c,
+    R vs1 (While e c) vs3 ->
+    (evalExp vs1 e = 0 /\ vs3 = vs1) \/
+    exists vs2, evalExp vs1 e <> 0 /\ R vs1 c vs2 /\ R vs2 (While e c) vs3.
+
+  Theorem evalCmd_coind : forall vs1 c vs2,
+    R vs1 c vs2 ->
+    evalCmd vs1 c vs2.
+  Proof.
+  cofix evalCmd_coind; intros; destruct c.
+  rewrite (AssignCase H); constructor.
+  destruct (SeqCase H) as [? [? ?]]; econstructor; eauto.
+  destruct (WhileCase H) as [[? ?] | [? [? [? ?]]]]; subst; econstructor; eauto.
+  Qed.
+End evalCmd_coind.
 
 
-      
-      
+Fixpoint optExp (e : exp) : exp :=
+  match e with
+    | Plus (Const 0) e => optExp e
+    | Plus e1 e2 => Plus (optExp e1) (optExp e2)
+    | _ => e
+  end.
 
-     
+Fixpoint optCmd (c : cmd) : cmd :=
+  match c with
+    | Assign v e => Assign v (optExp e)
+    | Seq c1 c2 => Seq (optCmd c1) (optCmd c2)
+    | While e c => While (optExp e) (optCmd c)
+  end.
+
+Lemma optExp_correct : forall vs e, evalExp vs (optExp e) = evalExp vs e.
+Proof.
+  intros. induction e; crush.
+  repeat (match goal with
+              | [ |- context[match ?E with Const _ => _ | _ => _ end] ] => destruct E
+              | [ |- context[match ?E with O => _ | S _ => _ end] ] => destruct E
+            end; crush).
+Qed.
+
+Hint Rewrite optExp_correct.
+
+Ltac finisher := match goal with
+                   | [ H : evalCmd _ _ _ |- _ ] => ((inversion H; [])
+                     || (inversion H; [|])); subst
+                 end; crush; eauto 10.
+
+Lemma optCmd_correct1 : forall vs1 c vs2, evalCmd vs1 c vs2
+  -> evalCmd vs1 (optCmd c) vs2.
+Proof.
+  intros; apply (evalCmd_coind (fun vs1 c' vs2 => exists c, evalCmd vs1 c vs2
+    /\ c' = optCmd c)); eauto; crush;
+    match goal with
+      | [ H : _ = optCmd ?E |- _ ] => destruct E; simpl in *; discriminate
+        || injection H; intros; subst
+    end; finisher.
+Qed.
+
+Lemma optCmd_correct2 : forall vs1 c vs2, evalCmd vs1 (optCmd c) vs2
+  -> evalCmd vs1 c vs2.
+  intros; apply (evalCmd_coind (fun vs1 c vs2 => evalCmd vs1 (optCmd c) vs2));
+    crush; finisher.
+Qed.
+
+Theorem optCmd_correct : forall vs1 c vs2, evalCmd vs1 (optCmd c) vs2
+  <-> evalCmd vs1 c vs2.
+  intuition; apply optCmd_correct1 || apply optCmd_correct2; assumption.
+Qed.
